theories/Compiler.v
@@ -200,7 +200,7 @@ Defined.
 
 Definition max_reg := 19%positive.
 
-Definition fromILF (s:stmt) :=
+Definition fromILF (s:stmt) o :=
   let s_eae := EAE.compile s in
   let sra := rename_apart_to_part FGS_even_fast_pos s_eae in
   let dcve := DCE Liveness.Imperative (fst sra) in
@@ -210,7 +210,7 @@ Definition fromILF (s:stmt) :=
   let rdom := (domain_add FG_fast_pres (empty_domain FG_fast_pres)
                          (getAnn (snd (spilled)))) in
   let ren2 := snd (renameApart FG_fast_pres rdom id (fst spilled)) in
-  let ras := rassign even_part_pos max_reg ren2
+  let ras := rassign even_part_pos o max_reg ren2
                     (snd (renameApart_live FG_fast_pres
                                            rdom
                                            id
@@ -278,8 +278,8 @@ Proof.
 Qed.
 
 
-Lemma fromILF_correct (s s':stmt) E (PM:LabelsDefined.paramsMatch s nil)
-      (OK:fromILF s = Success s')
+Lemma fromILF_correct (s s':stmt) E (PM:LabelsDefined.paramsMatch s nil) o
+      (OK:fromILF s o = Success s')
       (Def:defined_on (freeVars s) E)
   : sim F.state I.state bot3 SimExt (nil, E, s)
         (nil, (id [fromILF_fvl_ren s <-- fromILF_fvl s] ∘ E)
