theories/Infra/SmallestK.v
@@ -111,17 +111,20 @@ Proof.
 Qed.
 
 
-Lemma least_fresh_part_small1 X `{OrderedType X} p G x k
-  : (part_1 p) (least_fresh_part p G x)
+Lemma least_fresh_part_small1 X `{OrderedType X} p o G x k
+  : (part_1 p) (least_fresh_part p o G x)
     -> SetInterface.cardinal (filter (part_1 p) G) < k
-    -> least_fresh_part p G x \In of_list (ksmallest (part_1 p) k).
+    -> least_fresh_part p o G x \In of_list (ksmallest (part_1 p) k).
 Proof.
   unfold least_fresh_part in *. cases.
   + intros.
     eapply least_fresh_part_bounded; eauto.
   + intros.
     pose proof (least_fresh_P_p (part_2 p) G).
-  exfalso. eapply (part_disj p _ H0 H2).
+    exfalso.
+    unfold least_fresh_P_oracle in H0. cases in H0; dcr.
+    eapply (part_disj p _ H0 H3).
+    eapply (part_disj p _ H0 H2).
 Qed.
 
 Definition part_vars_bounded (p:inf_subset positive) k (x:positive) := p x -> (x ∈ of_list (ksmallest p k)).
@@ -129,11 +132,11 @@ Definition part_vars_bounded (p:inf_subset positive) k (x:positive) := p x -> (x
 Definition part_size_bounded X `{OrderedType X} (p:inf_subset X) k a :=
   SetInterface.cardinal (filter p a) <= k.
 
-Lemma fresh_list_stable_small (p:inf_partition positive) G k Z (ND:NoDupA eq Z)
+Lemma fresh_list_stable_small (p:inf_partition positive) o G k Z (ND:NoDupA eq Z)
   (BNDk : SetInterface.cardinal (filter (part_1 p) G) +
        SetInterface.cardinal (filter (part_1 p) (of_list Z)) <= k)
   : For_all (part_vars_bounded (part_1 p) k)
-            (of_list (fst (fresh_list_stable (stable_fresh_part p) G Z))).
+            (of_list (fst (fresh_list_stable (stable_fresh_part p o) G Z))).
 Proof.
   hnf; intros.
   eapply of_list_get_first in H; eauto; dcr. invc H1.
